identified and partially fixed the gap between vmem2reg and mem2reg 1) vmem2reg did not eliminate all phinodes [Aycock and Horspool, CC 200]    It only removed x = phi y1 l1, ... yn ln where yi = x or y    by subst x with y.
   It should also remove
     x = phi v1 l1, ... vn ln, where vi = x or v
   by subst x with v. Otherwise phis like x = phi undef l0 cannot be
   removed!

   IMPLEMENTED

2) We should not consider LLVM's debug intrinsics @llvm.dbg.declare as
   uses of promotable allocas. For maintaining debug info from src, LLVM
   does

   %p = alloca i32
   %t = bitcast i32* %p to {}*
   call ... @llvm.dbg.declare {}* %t ...

   Although %p is used by non-load/store, it is only used for debugging
   in this pattern. In semantics of @llvm.dbg.declare is no-op. So it is
   safe to promote %p.

   RULES: %p is promotable if
   a) %p is at entry
   b) %p is not used by non-load/store/bitcast
   c) if %p is used by only one bitcast, the bitcast result is used by
      only on @llvm.dbg.declare
   d) %p must be used by ld/st: The %p used only by @llvm.dbg.declare is
      really for debugging. LLVM does not want to remove it...

   IMPLEMENTED

   To prove, we need semantics and syntax for intrinsics. 
   
3) About pruned. The idea was prosed in Choi, Cytron and Ferrante,
   Automatic Construnction of Sparse Dara Flow Evaluation Graphs 
   (Sec 5.1), which only inserts phinodes for x in the blocks that x is
   alive w.r.t the standard liveness analysis.

   Concretely, LLVM only inserts phinodes for x at the blocks that uses
   x, and backward-transitively accesses x (reachable via prodecessors).

   So, this `might' equal to the minimal SSA + aggressive dead code
   elim(ADCE) for phinodes. Experimently the performance of -vmem2reg -adce
   and -mem2reg -adce are similar, and their generated code seems to be
   the same. I do not know if the pruned form = the minimal SSA + DCE.

   To fix the issue, we could
   a) at phinode-placement, we only place phis for x in alive blocks for
      x, rather than all reachable blocks, or
   b) implement an ADCE(DCE?) for x at the very end.
   
   For a), we should prove that the new placement + the original
   phi-elim = the pruned SSA. For b), it is not sure of minimal SSA +
   ADCE(DCE) = pruned SSA (the 3rd paragraph in Sec 5.1 of Choi's paper
   conjectures that they are the same)

4) In 3.0, mem2reg is not a top-level pass any more, which is contained
   by -scalarrepl(Scalar Replacement of Aggregates):

   The well-known scalar replacement of aggregates transformation. This
   transform breaks up alloca instructions of aggregate type (structure or
   array) into individual alloca instructions for each member if possible.
   Then, if possible, it transforms the individual alloca instructions into
   nice clean scalar SSA form.

   This combines a simple scalar replacement of aggregates algorithm with
   the mem2reg algorithm because often interact, especially for C++
   programs. As such, iterating between scalarrepl, then mem2reg until we
   run out of things to promote works well.

   Although we can still run -mem2reg manually, by default LLVM's
   scalarrepl pass will lower aggregates first and then mem2reg.

   So, the fix 1) 2) are only done in the 2.6 branch.



git-svn-id: https://webdav.seas.upenn.edu/svn/sol/vol@3717 eef5ea85-cc2e-0410-bd84-0fae1f012da8

src/Transforms/mem2reg.v
@@ -181,6 +181,7 @@ let '(bs', _, newpids) :=
        end) (List.rev bs) (nil, ex_ids, nil)) in
 (fdef_intro fh bs', newpids).
 
+
 Definition is_promotable (f:fdef) (pid:id) : bool :=
 let '(fdef_intro _ bs) := f in
 fold_left 
@@ -393,8 +394,8 @@ Definition elim_dead_st_fdef (pid:id) (f:fdef) : fdef :=
 let '(fdef_intro fh bs) := f in
 fdef_intro fh (List.map (elim_dead_st_block pid) bs).
 
-Definition macro_mem2reg_fdef_iter (f:fdef) (rd:list l) (succs preds:ATree.t (list l)) 
-  (dones:list id) : fdef * bool * list id := 
+Definition macro_mem2reg_fdef_iter (f:fdef) (rd:list l) 
+  (succs preds:ATree.t (list l)) (dones:list id) : fdef * bool * list id := 
 match getEntryBlock f with
 | Some (block_intro _ _ cs _) =>
     match find_promotable_alloca f cs dones with
@@ -428,33 +429,38 @@ let '(f, dones) := st in
 let '(f1, changed1, dones1) := mem2reg_fdef_iter f dt rd dones in
 if changed1 then inr _ (f1, dones1) else inl _ (f1, dones1).
 
-Fixpoint remove_redundancy (acc:ids) (ids0:ids) : ids :=
-match ids0 with
+Definition valueInListValueB (v0:value) (vs:list value) : bool :=
+List.fold_left (fun acc v => acc || valueEqB v0 v) vs false.
+
+Fixpoint remove_redundancy (acc:list value) (vs:list value) : list value :=
+match vs with
 | nil => acc
-| id1::ids0' => 
-    if (In_dec id_dec id1 acc) then remove_redundancy acc ids0'
-    else remove_redundancy (id1::acc) ids0'
+| v::vs' => 
+    if (valueInListValueB v acc) then remove_redundancy acc vs'
+    else remove_redundancy (v::acc) vs'
 end.
 
 Definition eliminate_phi (f:fdef) (pn:phinode): fdef * bool:=
 let '(insn_phi pid _ vls) := pn in 
-let vls' := unmake_list_value_l vls in
-let ops := values2ids (list_prj1 _ _ vls') in
-if (beq_nat (List.length ops) (List.length vls')) then
-  let ids0 := pid :: ops in
-  let ndp0 := remove_redundancy nil ids0 in
-  match ndp0 with
-  | id1::id2::nil =>
-    let pid := getPhiNodeID pn in
+let ndpvs := 
+  remove_redundancy nil (value_id pid::list_prj1 _ _ (unmake_list_value_l vls)) 
+in
+match ndpvs with
+| value_id id1 as v1::v2::nil =>
     if (id_dec pid id1) then 
-      (remove_fdef pid (isubst_fdef pid id2 f), true)
-    else if (id_dec pid id2) then 
-      (remove_fdef pid (isubst_fdef pid id1 f), true)
-    else (f, false)
-  | id1::nil => (remove_fdef id1 f, false)
-  | _ => (f, false)
-  end
-else (f, false).
+      (* if v1 is pid, then v2 cannot be pid*)
+      (remove_fdef pid (subst_fdef pid v2 f), true)
+    else  
+      (* if v1 isnt pid, then v2 must be pid*)
+      (remove_fdef pid (subst_fdef pid v1 f), true)
+| value_const _ as v1::_::nil =>
+    (* if v1 is const, then v2 must be pid*)
+    (remove_fdef pid (subst_fdef pid v1 f), true)
+| v1::nil => 
+    (* v1 must be pid, so pn:= pid = phi [pid, ..., pid] *)
+    (remove_fdef pid f, true)
+| _ => (f, false)
+end.
 
 Fixpoint eliminate_phis (f:fdef) (ps: phinodes): fdef * bool :=
 match ps with
@@ -482,16 +488,65 @@ if changed1 then inr _ f1 else inl _ f1.
 Parameter does_phi_elim : unit -> bool.
 Parameter does_macro_m2r : unit -> bool.
 
+Parameter is_llvm_dbg_declare : id -> bool.
+
+Definition remove_dbg_declare (pid:id) (f:fdef) : fdef :=
+let uses := find_uses_in_fdef pid f in
+let re :=List.fold_left
+  (fun acc i =>
+   match acc with
+   | None => None
+   | Some (bldst, ocid, orid) =>
+       match i with 
+       | insn_cmd (insn_load _ _ _ _) => Some (true, ocid, orid)
+       | insn_cmd (insn_store _ _ v _ _) => 
+           if valueEqB v (value_id pid) then None else Some (true, ocid, orid)
+       | insn_cmd (insn_cast cid castop_bitcast _ _ _) =>
+           match ocid with
+           | Some _ => 
+               (* not remove if used by multiple bitcast *)
+               None
+           | None =>
+               match find_uses_in_fdef cid f with
+               | insn_cmd 
+                   (insn_call rid _ _ _ (value_const (const_gid _ fid)) _)
+                   ::nil =>
+                   if is_llvm_dbg_declare fid then 
+                     Some (bldst, Some cid, Some rid)
+                   else None
+               | _ => None
+               end
+           end
+       | _ => None
+       end
+   end)
+  uses (Some (false, None, None)) in
+match re with
+| Some (true, Some cid, Some rid) => 
+    (* if pid is used by ld/st and a simple dbg *)
+    remove_fdef cid (remove_fdef rid f)
+| _ => f
+end.
+
+Fixpoint remove_dbg_declares (f:fdef) (cs:cmds) : fdef :=
+match cs with
+| nil => f
+| insn_alloca pid _ _ _ :: cs' =>
+    remove_dbg_declares (remove_dbg_declare pid f) cs'
+| _ :: cs' => remove_dbg_declares f cs'
+end.
+
 Definition mem2reg_fdef (f:fdef) : fdef :=
 match getEntryBlock f, reachablity_analysis f with
 | Some (block_intro root _ cs _), Some rd =>
   if print_reachablity rd then
     let '(f1, _) := 
       if (does_macro_m2r tt) then
-        let succs := successors f in
+        let f0 := remove_dbg_declares f cs in
+        let succs := successors f0 in
         let preds := make_predecessors succs in
         SafePrimIter.iterate _ 
-          (macro_mem2reg_fdef_step rd succs preds) (f, nil) 
+          (macro_mem2reg_fdef_step rd succs preds) (f0, nil) 
       else
         let b := bound_fdef f in
         let dts := dom_analyze f in
