src/Transforms/mem2reg_correct.v
@@ -837,6 +837,27 @@ Axiom fix_temporary_fdef_sim_wfS: forall f1 f2 Ps1 Ps2 los nts main VarArgs
     main VarArgs /\
   wf_system nil [module_intro los nts (Ps1 ++ product_fdef f2 :: Ps2)].
 
+Lemma remove_dbg_declares_sim_wfS: forall cs Ps1 Ps2 los nts main
+  VarArgs f,
+  (program_sim [module_intro los nts (Ps1 ++ product_fdef f :: Ps2)]
+               [module_intro los nts (Ps1 ++ product_fdef f :: Ps2)] main
+               VarArgs /\
+   wf_system nil [module_intro los nts (Ps1 ++ product_fdef f :: Ps2)]) ->
+  program_sim [module_intro los nts 
+                 (Ps1 ++ product_fdef (remove_dbg_declares f cs) :: Ps2)]
+               [module_intro los nts (Ps1 ++ product_fdef f :: Ps2)] main
+               VarArgs /\
+   wf_system nil 
+     [module_intro los nts 
+       (Ps1 ++ product_fdef (remove_dbg_declares f cs) :: Ps2)].
+Admitted.
+
+Lemma remove_dbg_declares_sim_reachablity_successors: forall f cs,
+  dtree.reachablity_analysis f 
+    = dtree.reachablity_analysis (remove_dbg_declares f cs) /\
+  successors f = successors (remove_dbg_declares f cs).
+Admitted.
+
 Lemma mem2reg_fdef_sim_wfS: forall (main : id) (VarArgs : list (GVsT DGVs))
   (los : layouts) (nts : namedts) (f : fdef) (Ps2 Ps1 : products)
   (HwfS : wf_system nil [module_intro los nts (Ps1 ++ product_fdef f :: Ps2)]),
@@ -850,15 +871,17 @@ Proof.
   intros.
   unfold mem2reg_fdef.
   remember (getEntryBlock f) as b. 
-  destruct b as [[root ps ts tmn]|]; auto using program_sim_refl.
+  destruct b as [[root ps cs tmn]|]; auto using program_sim_refl.
   remember (dtree.reachablity_analysis f) as R.
   destruct R as [rd|]; auto using program_sim_refl.
   rewrite print_reachablity_is_true.
   rewrite does_macro_m2r_is_true.
   remember (SafePrimIter.iterate (fdef * list id)
-                   (macro_mem2reg_fdef_step rd (successors f)
-                      (make_predecessors (successors f))) 
-                   (f, nil)) as R.
+                   (macro_mem2reg_fdef_step rd 
+                      (successors (remove_dbg_declares f cs))
+                      (make_predecessors 
+                        (successors (remove_dbg_declares f cs)))) 
+                   ((remove_dbg_declares f cs), nil)) as R.
   destruct R as [f1 dones]; auto using program_sim_refl.
   rewrite does_phi_elim_is_true.
   remember (fix_temporary_fdef (SafePrimIter.iterate fdef eliminate_step f1))
@@ -872,8 +895,13 @@ Proof.
           :: Ps2)]); auto; intros.
       eapply fix_temporary_fdef_sim_wfS; eauto.
       apply eliminate_phis_sim_wfS; auto.
-
+  apply program_sim_wfS_trans with (P2:=
+    [module_intro los nts 
+       (Ps1 ++ product_fdef (remove_dbg_declares f cs) :: Ps2)]); auto; intros.
     eapply macro_mem2reg_fdef_sim_wfS; eauto.
+      rewrite HeqR.
+      eapply remove_dbg_declares_sim_reachablity_successors; eauto.
+    apply remove_dbg_declares_sim_wfS; auto using program_sim_refl.
 Qed.
 
 Lemma mem2reg_run_sim_wfS_aux: forall (main : id) (VarArgs : list (GVsT DGVs))   
