src/Transforms/mem2reg.sh
@@ -1,0 +1,144 @@
+#!/bin/bash
+
+DIRS="../Interpreter/testcases/ ../Interpreter/testcases/llvm \
+	../Interpreter/testcases/softbound/"
+M2R=../_build/Transforms/main.native
+BC_DIR=./testcases/
+OC_DIR=./testcases/olden-ccured/
+OC_CASES="bh bisort em3d health mst perimeter power treeadd tsp"
+S95_DIR=./testcases/spec95-ccured/
+S95_CASES="129.compress 099.go 130.li 132.ijpeg"
+
+#PRE_OPT_FLAG="-disable-opt -raiseallocs -simplifycfg -domtree -domfrontier 
+#  -mem2reg 
+#  -globalopt -globaldce -ipconstprop -deadargelim -instcombine -simplifycfg 
+#  -basiccg -prune-eh -functionattrs -inline -simplify-libcalls -instcombine 
+#  -jump-threading -simplifycfg -domtree -domfrontier -scalarrepl -instcombine 
+#  -break-crit-edges -condprop -tailcallelim -simplifycfg -lowerswitch 
+#  -reassociate -domtree 
+#  -loops -loopsimplify -domfrontier -lcssa -loop-rotate -licm -lcssa 
+#  -loop-unswitch -instcombine -scalar-evolution -lcssa -iv-users -indvars 
+#  -loop-deletion -lcssa -loop-unroll -instcombine -lowerswitch -memdep"
+
+#SUF_OPT_FLAG="-disable-opt -memdep 
+#  -memcpyopt -sccp -instcombine -break-crit-edges -condprop -domtree -memdep -dse 
+#  -adce -simplifycfg -strip-dead-prototypes -print-used-types -deadtypeelim 
+#  -constmerge -preverify -domtree -verify"
+
+#PRE_LD_FLAG="-disable-opt -internalize -ipsccp -globalopt -constmerge 
+#  -deadargelim -instcombine -basiccg -inline -prune-eh -globalopt -globaldce 
+#  -basiccg -argpromotion -instcombine -jump-threading -domtree -domfrontier 
+#  -scalarrepl -basiccg -functionattrs -globalsmodref-aa -domtree -loops 
+#  -loopsimplify -domfrontier -licm -memdep"
+
+#SUF_LD_FLAG="-disable-opt -memdep -memcpyopt -dse -instcombine -jump-threading 
+#  -domtree -domfrontier -mem2reg -simplifycfg -globaldce -instcombine -simplifycfg 
+#  -adce -globaldce -preverify -domtree -verify"
+
+#OPT_FLAG="-disable-opt -raiseallocs -simplifycfg -domtree -domfrontier -mem2reg 
+#  -globalopt -globaldce -ipconstprop -deadargelim -instcombine -simplifycfg 
+#  -basiccg -prune-eh -functionattrs -inline -simplify-libcalls -instcombine 
+#  -jump-threading -simplifycfg -domtree -domfrontier -scalarrepl -instcombine 
+#  -break-crit-edges -condprop -tailcallelim -simplifycfg -reassociate -domtree 
+#  -loops -loopsimplify -domfrontier -lcssa -loop-rotate -licm -lcssa 
+#  -loop-unswitch -instcombine -scalar-evolution -lcssa -iv-users -indvars 
+#  -loop-deletion -lcssa -loop-unroll -instcombine -memdep 
+#  -gvn
+#  -memdep 
+#  -memcpyopt -sccp -instcombine -break-crit-edges -condprop -domtree -memdep -dse 
+#  -adce -simplifycfg -strip-dead-prototypes -print-used-types -deadtypeelim 
+#  -constmerge -preverify -domtree -verify"
+
+#NOGVN_OPT_FLAG="-disable-opt -raiseallocs -simplifycfg -domtree -domfrontier 
+#  -mem2reg 
+#  -globalopt -globaldce -ipconstprop -deadargelim -instcombine -simplifycfg 
+#  -basiccg -prune-eh -functionattrs -inline -simplify-libcalls -instcombine 
+#  -jump-threading -simplifycfg -domtree -domfrontier -scalarrepl -instcombine 
+#  -break-crit-edges -condprop -tailcallelim -simplifycfg -reassociate -domtree 
+#  -loops -loopsimplify -domfrontier -lcssa -loop-rotate -licm -lcssa 
+#  -loop-unswitch -instcombine -scalar-evolution -lcssa -iv-users -indvars 
+#  -loop-deletion -lcssa -loop-unroll -instcombine -memdep 
+#  -memdep 
+#  -memcpyopt -sccp -instcombine -break-crit-edges -condprop -domtree -memdep -dse 
+#  -adce -simplifycfg -strip-dead-prototypes -print-used-types -deadtypeelim 
+#  -constmerge -preverify -domtree -verify"
+
+#LD_FLAG="-disable-opt -internalize -ipsccp -globalopt -constmerge 
+#  -deadargelim -instcombine -basiccg -inline -prune-eh -globalopt -globaldce 
+#  -basiccg -argpromotion -instcombine -jump-threading -domtree -domfrontier 
+#  -scalarrepl -basiccg -functionattrs -globalsmodref-aa -domtree -loops 
+#  -loopsimplify -domfrontier -licm -memdep
+#  -gvn
+#  -memdep -memcpyopt -dse -instcombine -jump-threading 
+#  -domtree -domfrontier -mem2reg -simplifycfg -globaldce -instcombine -simplifycfg 
+#  -adce -globaldce -preverify -domtree -verify"
+LD_FLAG="-disable-opt -adce"
+
+PRE_OPT_FLAG="-disable-opt -raiseallocs -simplifycfg"
+M2R_OPT_FLAG="-disable-opt -raiseallocs -simplifycfg -domtree -domfrontier 
+              -mem2reg"
+
+Compiling ()
+{
+  echo -e $2": \c" ;
+
+  echo -e "Pre"; time opt -f $PRE_OPT_FLAG $1 -o $2"o.bc"
+
+  echo -e "Coq M2R"; time $M2R -mem2reg $2"o.bc" >& $2"a.ll"
+  llvm-as -f $2"a.ll" -o $2"a.bc"
+  echo -e "  LLVM ld"; time llvm-ld -native -lm $LD_FLAG $2"a.bc" -o $2"a.exe"
+
+  echo -e "Coq M2R no phielim"; time $M2R -mem2reg-no-phi-elim $2"o.bc" >& $2"c.ll"
+  llvm-as -f $2"c.ll" -o $2"c.bc"
+  echo -e "  LLVM ld"; time llvm-ld -native -lm $LD_FLAG $2"c.bc" -o $2"c.exe"
+ 
+  echo -e "LLVM ld"; time llvm-ld -native -lm $LD_FLAG $2"o.bc" -o $2"b.exe"
+
+  echo -e "LLVM M2R"; time opt -f $M2R_OPT_FLAG $1 -o $2"d.bc"
+  echo -e "  LLVM ld"; time llvm-ld -native -lm $LD_FLAG $2"d.bc" -o $2"d.exe"
+}
+
+Running ()
+{
+  echo -e $1" nopt: \c"; eval "time ./"$1"b.exe "$2" >& /dev/null"
+  echo -e $1" vm2r: \c"; eval "time ./"$1"a.exe "$2" >& /dev/null"
+  echo -e $1" vm2r noelim: \c"; eval "time ./"$1"c.exe "$2" >& /dev/null"
+  echo -e $1" m2r: \c"; eval "time ./"$1"d.exe "$2" >& /dev/null"
+}
+
+for name in ./testcases/*.ll; do 
+  echo -e $name": \c"  
+  llvm-as -f $name -o input.bc
+  $M2R -mem2reg input.bc
+  $M2R -mem2reg input.bc >& output.ll
+  llvm-as -f output.ll
+  llvm-ld output.bc -o test.exe
+  time ./test.exe
+done;
+
+for name in $OC_CASES; do 
+  Compiling $OC_DIR$name"/test.bc" $name
+done;
+Running "bh" "< ./testcases/olden-ccured/bh/slow_input";
+Running "bisort" "5000000 0";
+Running "em3d" "30000 300 50";
+Running "health" "8 250 1";
+Running "mst" "4000";
+Running "perimeter" "12 2000";
+Running "power" "";
+Running "treeadd" "24 10"; 
+Running "tsp" "2000000 0";
+
+for name in $S95_CASES; do 
+  Compiling $S95_DIR$name"/src/test.bc" $name
+done;
+Running "099.go" "100 15"
+#Running "130.li" "./testcases/spec95-ccured/130.li/src/ref.lsp";
+Running "129.compress" "< ./testcases/spec95-ccured/129.compress/src/slow_input.data";
+Running "132.ijpeg" "-image_file testcases/spec95-ccured/132.ijpeg/data/ref/input/vigo.ppm -compression.quality 90 -compression.optimize_coding 0 -compression.smoothing_factor 90 -difference.image 1 -difference.x_stride 10 -difference.y_stride 10 -verbose 1 -GO.findoptcomp"
+
+rm -f bisort* em3d* health* mst* treeadd* 129.compress* test-softbound.bc \
+  130.li* 099.go* tsp* bh* power* perimeter* 132.ijpeg* opt.bc input.* output.* \
+  test.exe test.exe.bc aa.db
+
+
